src/Ast/NamesAndLinearForms.dfy
@@ -1,0 +1,119 @@
+// This module defines two predicates that are used during resolution:
+//     * NameAlignment
+//     * LinearForm
+// along with some useful lemmas about these.
+
+module NamesAndLinearForms {
+  import Ast
+
+  export
+    reveals NameAlignment, LinearForm
+    provides LinearFormValues, LinearFormL2R, LinearFormR2L, NewNamePreservesLinearForm
+    provides DistinctConcat
+    provides Ast
+
+  ghost predicate NameAlignment(xMap: map<string, Ast.NamedDecl>) {
+    forall name <- xMap :: xMap[name].Name == name
+  }
+
+  ghost predicate LinearForm<X>(xMap: map<string, X>, xs: seq<X>) {
+    (set name <- xMap :: xMap[name]) == set x <- xs
+  }
+
+  lemma LinearFormValues<X>(xMap: map<string, X>, xs: seq<X>)
+    requires LinearForm(xMap, xs)
+    ensures xMap.Values == set x <- xs
+  {
+  }
+
+  lemma LinearFormL2R<X>(name: string, xMap: map<string, X>, xs: seq<X>)
+    requires LinearForm(xMap, xs) && name in xMap
+    ensures xMap[name] in xs
+  {
+    var lhs := set name <- xMap :: xMap[name];
+    var rhs := set x <- xs;
+    assert xMap[name] in lhs;
+    assert xMap[name] in rhs;
+  }
+
+  lemma LinearFormR2L<X>(x: X, xMap: map<string, X>, xs: seq<X>) returns (name: string)
+    requires LinearForm(xMap, xs) && x in xs
+    ensures name in xMap && xMap[name] == x
+  {
+    var lhs := set name <- xMap :: xMap[name];
+    var rhs := set x <- xs;
+    assert x in rhs;
+    assert x in lhs;
+    name :| name in xMap && xMap[name] == x;
+  }
+
+  lemma NewNamePreservesLinearForm(name: string, decl: Ast.NamedDecl, xMap: map<string, Ast.NamedDecl>, xs: seq<Ast.NamedDecl>)
+    requires NameAlignment(xMap)
+    requires LinearForm(xMap, xs)
+    requires name !in xMap
+    requires decl.Name == name
+    ensures forall i :: 0 <= i < |xs| ==> xs[i].Name != name
+    ensures LinearForm(xMap[name := decl], xs + [decl])
+  {
+    forall i | 0 <= i < |xs|
+      ensures xs[i].Name != name
+    {
+      // From the definition of LinearForm:
+      var lhs := set xName <- xMap :: xMap[xName];
+      var rhs := set x <- xs;
+      assert lhs == rhs; // by LinearForm(xMap, xs)
+
+      var x := xs[i];
+      assert x in xs;
+      assert x in rhs;
+      assert x in lhs;
+      var xName :| xName in xMap && xMap[xName] == x;
+      assert xMap[xName].Name == xName;
+      assert xName != name; // since "xName in xMap" and "name !in xMap"
+    }
+
+    var xMap', xs' := xMap[name := decl], xs + [decl];
+    var n := |xs|;
+    calc {
+      (set xName <- xMap' :: xMap'[xName]);
+      (set xName <- xMap :: xMap'[xName]) + {xMap'[name]};
+      { assert name !in xMap; }
+      (set xName <- xMap :: xMap[xName]) + {decl};
+      { assert LinearForm(xMap, xs); }
+      (set x <- xs) + {decl};
+      { assert xs == xs'[..n] && xs'[n] == decl; }
+      (set x <- xs'[..n]) + {xs'[n]};
+      (set x <- xs');
+    }
+  }
+
+  lemma DistinctConcat(xMap: map<string, Ast.NamedDecl>, xs: seq<Ast.NamedDecl>, yMap: map<string, Ast.NamedDecl>, ys: seq<Ast.NamedDecl>)
+    requires LinearForm(xMap, xs) && LinearForm(yMap, ys)
+    requires NameAlignment(xMap) && NameAlignment(yMap)
+    requires xMap.Keys !! yMap.Keys
+    requires Ast.NamedDecl.Distinct(xs) && Ast.NamedDecl.Distinct(ys)
+    ensures Ast.NamedDecl.Distinct(xs + ys)
+  {
+    var decls := xs + ys;
+    forall i, j | 0 <= i < j < |decls|
+      ensures decls[i].Name != decls[j].Name
+    {
+      var n := |xs|;
+      assert decls[..n] == xs && decls[n..] == ys;
+      if j < n {
+        assert decls[i] in xs && decls[j] in xs;
+      } else if n <= i {
+        assert decls[i] in ys && decls[j] in ys;
+      } else {
+        assert decls[i].Name in xMap by {
+          var name := LinearFormR2L(decls[i], xMap, xs);
+          assert xMap[name].Name == name; // by NameAlignment
+        }
+        assert decls[j].Name in yMap by {
+          var name := LinearFormR2L(decls[j], yMap, ys);
+          assert yMap[name].Name == name; // by NameAlignment
+        }
+      }
+    }
+  }
+}
